steel/Zeta.Steel.Verifier.fst
@@ -22,12 +22,13 @@ open Zeta.Steel.EpochHashes
 module Application = Zeta.Steel.Application
 #push-options "--ide_id_info_off"
 
-
 let spec_parser_consumes (l:bytes)
   : Lemma (match LogEntry.spec_parser_log_entry l with
            | None -> True
            | Some (_, n) -> n > 0)
-  = admit()
+  = match LogEntry.spec_parser_log_entry l with
+    | None -> ()
+    | _ -> LogEntry.Spec.spec_parser_log_entry_consumes_at_least_one_byte l
 
 let rec parse_full_log' (l:bytes)
                         (offset:nat { offset <= Seq.length l })
@@ -77,19 +78,22 @@ let fail (#p:prop)
     elim_pure _;
     ()
 
-let intro_nout_bytes //(#o:_)
+let intro_nout_bytes (#o:_)
                      (tsm tsm':M.thread_state_model)
                      (out_bytes:erased bytes)
-  : ST unit
+                     (out_offset:U32.t { U32.v out_offset <= Seq.length out_bytes })
+  : STGhost unit o
     emp
-    (fun _ -> pure (Application.n_out_bytes tsm tsm' 0ul out_bytes out_bytes))
+    (fun _ -> pure (Application.n_out_bytes tsm tsm' out_offset 0ul out_bytes out_bytes))
     (requires Application.delta_out_bytes tsm tsm' == Seq.empty)
     (ensures fun _ -> True)
-  = admit__()
+  = intro_pure (Application.n_out_bytes tsm tsm' out_offset 0ul out_bytes out_bytes)
+
 
 let verify_log_entry_post (tsm:M.thread_state_model)
                           (t:thread_state_t)
                           (out_bytes0:bytes)
+                          (out_offset:U32.t)
                           (out:A.array U8.t) //out array, to write outputs
                           (aeh:AEH.aggregate_epoch_hashes) //lock & handle to the aggregate state
                           (le:LogEntry.log_entry)
@@ -111,13 +115,14 @@ let verify_log_entry_post (tsm:M.thread_state_model)
            thread_state_inv t tsm' `star` //tsm' is the new state of the thread
            array_pts_to out out_bytes1 `star`  //the out array contains out_bytes
            TLM.tid_pts_to aeh.mlogs tsm.thread_id full tsm'.processed_entries false `star` //my contributions are updated
-           pure (Application.n_out_bytes tsm tsm' n_out out_bytes0 out_bytes1))
+           pure (Application.n_out_bytes tsm tsm' out_offset n_out out_bytes0 out_bytes1))
 
 let success (#o:_)
             (#tsm:M.thread_state_model)
             (t:thread_state_t)
             (aeh:AEH.aggregate_epoch_hashes) //lock & handle to the aggregate state
             (#out_bytes0 #out_bytes1:erased _)
+            (out_offset:U32.t)
             (out:A.array U8.t)
             (le:log_entry)
             (n_out:U32.t)
@@ -125,22 +130,23 @@ let success (#o:_)
     (thread_state_inv t (M.verify_step_model tsm le) `star`
      TLM.tid_pts_to aeh.mlogs tsm.thread_id full (M.verify_step_model tsm le).processed_entries false `star`
      array_pts_to out out_bytes1 `star`
-     pure (Application.n_out_bytes tsm (M.verify_step_model tsm le) n_out out_bytes0 out_bytes1))
+     pure (Application.n_out_bytes tsm (M.verify_step_model tsm le) out_offset n_out out_bytes0 out_bytes1))
     (fun _ ->
-      verify_log_entry_post tsm t out_bytes0 out aeh le (Some n_out))
+      verify_log_entry_post tsm t out_bytes0 out_offset out aeh le (Some n_out))
   = let tsm' = M.verify_step_model tsm le in
     intro_exists_erased out_bytes1
        (fun (out_bytes1:Seq.seq U8.t) ->
          thread_state_inv t tsm' `star` //tsm' is the new state of the thread
          array_pts_to out out_bytes1 `star`  //the out array contains out_bytes
          TLM.tid_pts_to aeh.mlogs tsm.thread_id full tsm'.processed_entries false `star` //my contributions are updated
-         pure (Application.n_out_bytes tsm tsm' n_out out_bytes0 out_bytes1))
+         pure (Application.n_out_bytes tsm tsm' out_offset n_out out_bytes0 out_bytes1))
 
 
 val verify_entry_cases (#tsm:M.thread_state_model)
                        (t:thread_state_t) //handle to the thread state
                        (#outlen:U32.t)
                        (#out_bytes0:erased bytes)
+                       (out_offset:U32.t { U32.v out_offset <= Seq.length out_bytes0 })
                        (out:larray U8.t outlen) //out array, to write outputs
                        (aeh:AEH.aggregate_epoch_hashes) //lock & handle to the aggregate state
                        (le:LogEntry.log_entry)
@@ -149,28 +155,31 @@ val verify_entry_cases (#tsm:M.thread_state_model)
     (thread_state_inv t (update_if b tsm (M.verify_step_model tsm le)) `star`
      TLM.tid_pts_to aeh.mlogs tsm.thread_id full tsm.processed_entries false `star`
      array_pts_to out out_bytes0)
-    (fun res -> verify_log_entry_post tsm t out_bytes0 out aeh le res)
+    (fun res -> verify_log_entry_post tsm t out_bytes0 out_offset out aeh le res)
     (requires
       not (VerifyEpoch? le) /\ not (RunApp? le) /\
       not tsm.failed)
     (ensures fun _ -> True)
+
 //fusing val and let leads to errors
 let verify_entry_cases (#tsm:M.thread_state_model)
                        (t:thread_state_t) //handle to the thread state
                        (#outlen:U32.t)
                        (#out_bytes0:erased bytes)
+                       (out_offset:U32.t { U32.v out_offset <= Seq.length out_bytes0 })
                        (out:larray U8.t outlen) //out array, to write outputs
                        (aeh:AEH.aggregate_epoch_hashes) //lock & handle to the aggregate state
                        (le:LogEntry.log_entry)
                        (b:bool)
   = compat_with_any_anchor_of_le tsm.processed_entries le;
     TLM.update_tid_log aeh.mlogs tsm.thread_id tsm.processed_entries (M.verify_step_model tsm le).processed_entries;
-    intro_nout_bytes tsm (M.verify_step_model tsm le) out_bytes0;
+    Application.delta_out_bytes_not_runapp tsm le;
+    intro_nout_bytes tsm (M.verify_step_model tsm le) out_bytes0 out_offset;
     if b
     then (
       rewrite (thread_state_inv t _)
               (thread_state_inv t (M.verify_step_model tsm le));
-      success t aeh out le 0ul;
+      success t aeh out_offset out le 0ul;
       return (Some 0ul)
     )
     else (
@@ -180,43 +189,34 @@ let verify_entry_cases (#tsm:M.thread_state_model)
       return None
     )
 
-val verify_log_entry (#tsm:M.thread_state_model)
+#push-options "--query_stats --fuel 0 --ifuel 1 --z3rlimit_factor 3"
+let verify_log_entry (#tsm:M.thread_state_model)
                      (t:thread_state_t) //handle to the thread state
                      (#outlen:U32.t)
-                     (#outbytes0:erased bytes)
+                     (#out_bytes:erased bytes)
+                     (out_offset:U32.t { U32.v out_offset <= Seq.length out_bytes })
                      (out:larray U8.t outlen) //out array, to write outputs
                      (aeh:AEH.aggregate_epoch_hashes) //lock & handle to the aggregate state
                      (le:LogEntry.log_entry)
   : ST (option U32.t)
     (//precondition
-      thread_state_inv t tsm `star` //thread state is initially tsm
-      array_pts_to out outbytes0 `star` //we have permission to out, don't care what it contains
-      TLM.tid_pts_to aeh.mlogs tsm.thread_id full tsm.processed_entries false //and the global state contains this thread's entries
-    )
+      thread_state_inv t tsm `star`
+      array_pts_to out out_bytes `star`
+      TLM.tid_pts_to aeh.mlogs tsm.thread_id full tsm.processed_entries false)
     (fun res -> //postcondition
-      verify_log_entry_post tsm t outbytes0 out aeh le res)
+      verify_log_entry_post tsm t out_bytes out_offset out aeh le res)
     (requires not tsm.failed /\
               not (RunApp? le))
     (ensures fun _ -> True)
-
-#push-options "--query_stats --fuel 0 --ifuel 1 --z3rlimit_factor 3"
-
-let verify_log_entry (#tsm:M.thread_state_model)
-                     (t:thread_state_t) //handle to the thread state
-                     (#outlen:U32.t)
-                     (#out_bytes:erased bytes)
-                     (out:larray U8.t outlen) //out array, to write outputs
-                     (aeh:AEH.aggregate_epoch_hashes) //lock & handle to the aggregate state
-                     (le:LogEntry.log_entry)
    = match le with
      | VerifyEpoch ->
        let b = VerifierSteps.verify_epoch t aeh in
-       intro_nout_bytes tsm (M.verify_step_model tsm le) out_bytes;
+       intro_nout_bytes tsm (M.verify_step_model tsm le) out_bytes out_offset;
        if b
        then (
          rewrite (thread_state_inv t _)
                  (thread_state_inv t (M.verify_step_model tsm le));
-         success t aeh out le 0ul;
+         success t aeh out_offset out le 0ul;
          return (Some 0ul)
        )
        else (
@@ -227,39 +227,37 @@ let verify_log_entry (#tsm:M.thread_state_model)
        )
 
      | _ ->
-       // compat_with_any_anchor_of_le tsm.processed_entries le;
-       // TLM.update_tid_log aeh.mlogs tsm.thread_id tsm.processed_entries (M.verify_step_model tsm le).processed_entries;
-       // intro_nout_bytes tsm (M.verify_step_model tsm le) out_bytes;
        match le with
        | AddM s s' r ->
          let b = VerifierSteps.vaddm t s s' r in
-         verify_entry_cases t out aeh le b
+         verify_entry_cases t out_offset out aeh le b
 
        | AddB s ts tid r ->
          let b = VerifierSteps.vaddb t s ts tid r in
-         verify_entry_cases t out aeh le b
+         verify_entry_cases t out_offset out aeh le b
 
        | EvictM pl ->
          VerifierSteps.vevictm t pl.s pl.s';
-         verify_entry_cases t out aeh le true
+         verify_entry_cases t out_offset out aeh le true
 
        | EvictB pl ->
          let b = VerifierSteps.vevictb t pl.s pl.t in
-         verify_entry_cases t out aeh le b
+         verify_entry_cases t out_offset out aeh le b
 
        | EvictBM pl ->
          let b = VerifierSteps.vevictbm t pl.s pl.s' pl.t in
-         verify_entry_cases t out aeh le b
+         verify_entry_cases t out_offset out aeh le b
 
        | NextEpoch ->
          let b = VerifierSteps.nextepoch t in
-         verify_entry_cases t out aeh le true
+         verify_entry_cases t out_offset out aeh le true
 
 let verify_step_post (tsm:M.thread_state_model)
                      (t:thread_state_t) //handle to the thread state
                      (log_bytes:bytes)
                      (log_pos:U32.t{U32.v log_pos <= Seq.length log_bytes})
                      (out_bytes:bytes)
+                     (out_offset:U32.t)
                      (out:A.array U8.t) //out array, to write outputs
                      (aeh:AEH.aggregate_epoch_hashes) //lock & handle to the aggregate state
                      ([@@@smt_fallback] res:verify_result)
@@ -281,12 +279,12 @@ let verify_step_post (tsm:M.thread_state_model)
       pure (Verify_entry_failure?.log_pos res == log_pos) `star`
       (match (LogEntry.spec_parser_log_entry (Parser.bytes_from log_bytes log_pos)) with
        | None -> pure False
-       | Some (le, _) -> verify_log_entry_post tsm t out_bytes out aeh le None)
+       | Some (le, _) -> verify_log_entry_post tsm t out_bytes out_offset out aeh le None)
 
    | Verify_success read wrote ->
       exists_ (fun le ->
         pure (LogEntry.maybe_parse_log_entry log_bytes log_pos == Some (le, U32.v read)) `star`
-        verify_log_entry_post tsm t out_bytes out aeh le (Some wrote))
+        verify_log_entry_post tsm t out_bytes out_offset out aeh le (Some wrote))
 
 let intro_verify_step_post_parsing_failure
                      (#o:_)
@@ -295,6 +293,7 @@ let intro_verify_step_post_parsing_failure
                      (log_bytes:erased bytes)
                      (log_pos:U32.t{U32.v log_pos <= Seq.length log_bytes})
                      (out_bytes:bytes)
+                     (out_offset:U32.t)
                      (out:A.array U8.t) //out array, to write outputs
                      (aeh:AEH.aggregate_epoch_hashes) //lock & handle to the aggregate state
   : STGhost unit o
@@ -302,7 +301,7 @@ let intro_verify_step_post_parsing_failure
      TLM.tid_pts_to aeh.mlogs tsm.thread_id full tsm.processed_entries false `star`
      array_pts_to out out_bytes)
     (fun _ ->
-      verify_step_post tsm t log_bytes log_pos out_bytes out aeh (Parsing_failure log_pos))
+      verify_step_post tsm t log_bytes log_pos out_bytes out_offset out aeh (Parsing_failure log_pos))
     (requires
       LogEntry.spec_parser_log_entry (Parser.bytes_from log_bytes log_pos) == None)
     (ensures fun _ -> True)
@@ -321,6 +320,7 @@ let intro_verify_step_post_app_failure
                      (log_bytes:erased bytes)
                      (log_pos:U32.t{U32.v log_pos <= Seq.length log_bytes})
                      (out_bytes:bytes)
+                     (out_offset:U32.t)
                      (out:A.array U8.t)
                      (aeh:AEH.aggregate_epoch_hashes) //lock & handle to the aggregate state
   : STGhostT unit o
@@ -328,7 +328,7 @@ let intro_verify_step_post_app_failure
      TLM.tid_pts_to aeh.mlogs tsm.thread_id full tsm.processed_entries false `star`
      array_pts_to out out_bytes)
     (fun _ ->
-      verify_step_post tsm t log_bytes log_pos out_bytes out aeh (App_failure log_pos))
+      verify_step_post tsm t log_bytes log_pos out_bytes out_offset out aeh (App_failure log_pos))
   = rewrite (thread_state_inv t tsm `star`
              TLM.tid_pts_to aeh.mlogs tsm.thread_id full tsm.processed_entries false `star`
              array_pts_to out out_bytes)
@@ -341,20 +341,21 @@ let intro_verify_step_post_verify_failure
                      (log_bytes:erased bytes)
                      (log_pos:U32.t{U32.v log_pos <= Seq.length log_bytes})
                      (out_bytes:bytes)
+                     (out_offset:U32.t)
                      (out:A.array U8.t)
                      (aeh:AEH.aggregate_epoch_hashes) //lock & handle to the aggregate state
                      (le: log_entry)
   : STGhost unit o
-    (verify_log_entry_post tsm t out_bytes out aeh le None)
+    (verify_log_entry_post tsm t out_bytes out_offset out aeh le None)
     (fun _ ->
-      verify_step_post tsm t log_bytes log_pos out_bytes out aeh (Verify_entry_failure log_pos))
+      verify_step_post tsm t log_bytes log_pos out_bytes out_offset out aeh (Verify_entry_failure log_pos))
     (requires
        (match (LogEntry.spec_parser_log_entry (Parser.bytes_from log_bytes log_pos)) with
        | None -> False
        | Some (le', n') -> le == le'))
     (ensures fun _ -> True)
   = intro_pure (Verify_entry_failure?.log_pos (Verify_entry_failure log_pos) == log_pos);
-    rewrite (pure _ `star` (verify_log_entry_post tsm t out_bytes out aeh le None))
+    rewrite (pure _ `star` (verify_log_entry_post tsm t out_bytes out_offset out aeh le None))
             _
 
 let intro_verify_step_post_verify_success
@@ -364,15 +365,16 @@ let intro_verify_step_post_verify_success
                      (log_bytes:erased bytes)
                      (log_pos:U32.t{U32.v log_pos <= Seq.length log_bytes})
                      (out_bytes:bytes)
+                     (out_offset:U32.t)
                      (out:A.array U8.t) //out array, to write outputs
                      (aeh:AEH.aggregate_epoch_hashes) //lock & handle to the aggregate state
                      (le: log_entry)
                      (n_read:U32.t)
                      (n_written:U32.t)
   : STGhost unit o
-    (verify_log_entry_post tsm t out_bytes out aeh le (Some n_written))
+    (verify_log_entry_post tsm t out_bytes out_offset out aeh le (Some n_written))
     (fun _ ->
-      verify_step_post tsm t log_bytes log_pos out_bytes out aeh (Verify_success n_read n_written))
+      verify_step_post tsm t log_bytes log_pos out_bytes out_offset out aeh (Verify_success n_read n_written))
     (requires
        LogEntry.can_parse_log_entry log_bytes log_pos /\
        LogEntry.spec_parse_log_entry log_bytes log_pos == (le, U32.v n_read))
@@ -380,7 +382,7 @@ let intro_verify_step_post_verify_success
   = intro_pure (LogEntry.maybe_parse_log_entry log_bytes log_pos == Some (le, U32.v n_read));
     intro_exists le (fun le ->
       pure (LogEntry.maybe_parse_log_entry log_bytes log_pos == Some (le, U32.v n_read)) `star`
-      verify_log_entry_post tsm t out_bytes out aeh le (Some n_written))
+      verify_log_entry_post tsm t out_bytes out_offset out aeh le (Some n_written))
 
 let intro_verify_step_post_runapp_success
                      (#o:_)
@@ -390,33 +392,32 @@ let intro_verify_step_post_runapp_success
                      (log_pos:U32.t{U32.v log_pos <= Seq.length log_bytes})
                      (pl: runApp_payload)
                      (out_bytes:bytes)
+                     (out_offset:U32.t)
                      (out:A.array U8.t)
                      (aeh:AEH.aggregate_epoch_hashes) //lock & handle to the aggregate state
                      (n_read:U32.t)
                      (n_written:U32.t)
                      (res:Application.verify_runapp_result)
   : STGhost unit o
-    (Application.verify_runapp_entry_post tsm t pl out_bytes out res `star`
+    (Application.verify_runapp_entry_post tsm t pl out_bytes out_offset out res `star`
      TLM.tid_pts_to aeh.mlogs tsm.thread_id full tsm.processed_entries false)
     (fun _ ->
-      verify_step_post tsm t log_bytes log_pos out_bytes out aeh (Verify_success n_read n_written))
+      verify_step_post tsm t log_bytes log_pos out_bytes out_offset out aeh (Verify_success n_read n_written))
     (requires
       res == Application.Run_app_success n_written /\ not tsm.failed /\
       LogEntry.can_parse_log_entry log_bytes log_pos /\
       LogEntry.spec_parse_log_entry log_bytes log_pos == (RunApp pl, U32.v n_read))
     (ensures fun _ -> True)
-  = rewrite (Application.verify_runapp_entry_post tsm t pl out_bytes out res)
-            (Application.verify_runapp_entry_post tsm t pl out_bytes out (Application.Run_app_success n_written));
+  = rewrite (Application.verify_runapp_entry_post tsm t pl out_bytes out_offset out res)
+            (Application.verify_runapp_entry_post tsm t pl out_bytes out_offset out (Application.Run_app_success n_written));
     let out_bytes' = elim_exists () in
-    elim_pure _;
     assert_ (thread_state_inv t (M.verify_step_model tsm (RunApp pl)));
     assert_ (array_pts_to out out_bytes');
     compat_with_any_anchor_of_le tsm.processed_entries (RunApp pl);
     TLM.update_tid_log aeh.mlogs tsm.thread_id tsm.processed_entries (M.verify_step_model tsm (RunApp pl)).processed_entries;
-    intro_pure (Application.n_out_bytes tsm (M.verify_step_model tsm (RunApp pl)) n_written  out_bytes out_bytes');
-    success t aeh out (RunApp pl) n_written;
-    assert_ (verify_log_entry_post tsm t out_bytes out aeh (RunApp pl) (Some n_written));
-    intro_verify_step_post_verify_success t log_bytes log_pos out_bytes out aeh (RunApp pl) n_read n_written
+    success t aeh out_offset out (RunApp pl) n_written;
+    assert_ (verify_log_entry_post tsm t out_bytes out_offset out aeh (RunApp pl) (Some n_written));
+    intro_verify_step_post_verify_success t log_bytes log_pos out_bytes out_offset out aeh (RunApp pl) n_read n_written
 
 val verify_step (#tsm:M.thread_state_model)
                 (t:thread_state_t) //handle to the thread state
@@ -427,7 +428,7 @@ val verify_step (#tsm:M.thread_state_model)
                 (log:larray U8.t len) //concrete log
                 (#outlen:U32.t)
                 (#out_bytes:erased bytes)
-                (out_pos:U32.t{U32.v out_pos <= U32.v outlen})
+                (out_offset:U32.t{ U32.v out_offset <= Seq.length out_bytes })
                 (out:larray U8.t outlen) //out array, to write outputs
                 (aeh:AEH.aggregate_epoch_hashes) //lock & handle to the aggregate state
   : ST verify_result
@@ -439,7 +440,7 @@ val verify_step (#tsm:M.thread_state_model)
     )
     (fun res -> //postcondition
       A.pts_to log log_perm log_bytes `star` //log contents didn't change
-      verify_step_post tsm t log_bytes log_pos out_bytes out aeh res)
+      verify_step_post tsm t log_bytes log_pos out_bytes out_offset out aeh res)
     (requires not tsm.failed)
     (ensures fun _ -> True)
 
@@ -454,7 +455,7 @@ let verify_step (#tsm:M.thread_state_model)
                 (log:larray U8.t len) //concrete log
                 (#out_len:U32.t)
                 (#out_bytes:erased bytes)
-                (out_pos:U32.t{U32.v out_pos <= U32.v out_len})
+                (out_offset:U32.t{U32.v out_offset <= Seq.length out_bytes})
                 (out:larray U8.t out_len) //out array, to write outputs
                 (aeh:AEH.aggregate_epoch_hashes) //lock & handle to the aggregate state
     = A.pts_to_length log _;
@@ -462,7 +463,7 @@ let verify_step (#tsm:M.thread_state_model)
       let res = LogEntry.parser_log_entry len log_pos U32.(len -^ log_pos) log in
       match res with
       | None ->
-        intro_verify_step_post_parsing_failure t log_bytes log_pos out_bytes out aeh;
+        intro_verify_step_post_parsing_failure t log_bytes log_pos out_bytes out_offset out aeh;
         return (Parsing_failure log_pos)
 
       | Some (le, read) ->
@@ -474,79 +475,44 @@ let verify_step (#tsm:M.thread_state_model)
             let pl_pos = log_pos `U32.add` pl_pos0 in
             Application.run_app_function
               len pl pl_pos log
-              out_len 0ul out
+              out_len out_offset out
               t
           in
+          // assert_ (Application.verify_runapp_entry_post tsm t pl out_bytes out_offset out app_res);
           begin
           match app_res with
           | Application.Run_app_parsing_failure
           | Application.Run_app_verify_failure ->
-            rewrite (Application.verify_runapp_entry_post _ _ _ _ _ _)
+            rewrite (Application.verify_runapp_entry_post tsm t pl out_bytes out_offset out app_res)
                     (thread_state_inv t tsm `star`
                      array_pts_to out out_bytes);
-            intro_verify_step_post_app_failure t log_bytes log_pos out_bytes out aeh;
+            intro_verify_step_post_app_failure t log_bytes log_pos out_bytes out_offset out aeh;
             return (App_failure log_pos)
 
           | Application.Run_app_success written ->
-//            assert_ (Application.verify_runapp_entry_post tsm t log_pos log_bytes out_bytes out app_res);
-            let _ = intro_verify_step_post_runapp_success t log_bytes log_pos pl out_bytes out aeh read written app_res in
+            let _ = intro_verify_step_post_runapp_success
+                        t log_bytes log_pos pl
+                        out_bytes out_offset out aeh read written app_res in
             return (Verify_success read written)
           end
 
         | _ ->
-          let b = verify_log_entry t out aeh le in
+          let b = verify_log_entry t out_offset out aeh le in
           match b with
           | None ->
-            rewrite (verify_log_entry_post tsm t out_bytes out aeh le b)
-                    (verify_log_entry_post tsm t out_bytes out aeh le None);
-            intro_verify_step_post_verify_failure t log_bytes log_pos out_bytes out aeh le;
+            rewrite (verify_log_entry_post tsm t out_bytes out_offset out aeh le b)
+                    (verify_log_entry_post tsm t out_bytes out_offset out aeh le None);
+            intro_verify_step_post_verify_failure t log_bytes log_pos out_bytes out_offset out aeh le;
             return (Verify_entry_failure log_pos)
 
           | Some written ->
-            rewrite (verify_log_entry_post tsm t out_bytes out aeh le b)
-                    (verify_log_entry_post tsm t out_bytes out aeh le (Some written));
-            intro_verify_step_post_verify_success t log_bytes log_pos out_bytes out aeh le read written;
+            rewrite (verify_log_entry_post tsm t out_bytes out_offset out aeh le b)
+                    (verify_log_entry_post tsm t out_bytes out_offset out aeh le (Some written));
+            intro_verify_step_post_verify_success t log_bytes log_pos out_bytes out_offset out aeh le read written;
             return (Verify_success read written)
 
 
 ////////////////////////////////////////////////////////////////////////////////
-
-// let some_failure (t:thread_state_t) //handle to the thread state
-//                  (out:A.array U8.t)
-//                  (aeh:AEH.aggregate_epoch_hashes) //lock & handle to the aggregate state
-//   : vprop
-//   = exists_ (thread_state_inv t) `star`
-//     exists_ (fun entries -> TLM.tid_pts_to aeh.mlogs (VerifierTypes.thread_id t) full entries false) `star`
-//     exists_ (array_pts_to out)
-
-// let verify_post (tsm:M.thread_state_model)
-//                 (t:thread_state_t) //handle to the thread state
-//                 (log_bytes:bytes)
-//                 (out_bytes:bytes)
-//                 (out:A.array U8.t)
-//                 (aeh:AEH.aggregate_epoch_hashes) //lock & handle to the aggregate state
-//                 ([@@@smt_fallback] res:verify_result)
-//  : vprop
-//  = match res with
-//    | Parsing_failure log_pos ->
-//       pure (~ (LogEntry.can_parse_log_entry log_bytes log_pos) ) `star`
-//       some_failure t out aeh
-
-//    | App_failure _ ->
-//       some_failure t out aeh
-
-//    | Verify_entry_failure _ ->
-//       some_failure t out aeh
-
-//    | Verify_success read wrote ->
-//      exists_ (fun log ->
-//        let tsm' = M.verify_model tsm log in
-//        pure (parse_log_up_to log_bytes (U32.v read) == Some log) `star`
-//        thread_state_inv t tsm' `star` //tsm' is the new state of the thread
-//        TLM.tid_pts_to aeh.mlogs tsm'.thread_id full tsm'.processed_entries false `star` //my contributions are updated
-//        exists_ (fun (out_bytes1:Seq.seq U8.t) ->
-//            array_pts_to out out_bytes1 `star`  //the out array contains out_bytes
-//            pure (Application.n_out_bytes tsm tsm' wrote out_bytes out_bytes1)))
 
 
 
@@ -557,11 +523,12 @@ let elim_verify_step_post_parsing_failure
                      (#log_bytes:bytes)
                      (#log_pos:U32.t{U32.v log_pos <= Seq.length log_bytes})
                      (#out_bytes:bytes)
+                     (#out_offset:U32.t)
                      (#out:A.array U8.t) //out array, to write outputs
                      (#aeh:AEH.aggregate_epoch_hashes) //lock & handle to the aggregate state
                      (loc:U32.t)
    : STGhost unit o
-     (verify_step_post tsm t log_bytes log_pos out_bytes out aeh (Parsing_failure loc))
+     (verify_step_post tsm t log_bytes log_pos out_bytes out_offset out aeh (Parsing_failure loc))
      (fun _ ->
         thread_state_inv t tsm `star`
         TLM.tid_pts_to aeh.mlogs tsm.thread_id full tsm.processed_entries false `star`
@@ -571,7 +538,7 @@ let elim_verify_step_post_parsing_failure
        LogEntry.spec_parser_log_entry (Parser.bytes_from log_bytes log_pos) == None /\
        loc == log_pos)
    = rewrite
-        (verify_step_post tsm t log_bytes log_pos out_bytes out aeh (Parsing_failure loc))
+        (verify_step_post tsm t log_bytes log_pos out_bytes out_offset out aeh (Parsing_failure loc))
         (pure (LogEntry.spec_parser_log_entry (Parser.bytes_from log_bytes log_pos) == None /\
                loc == log_pos) `star`
          thread_state_inv t tsm `star`
@@ -611,14 +578,15 @@ let elim_verify_step_post_app_failure
                      (#log_bytes:bytes)
                      (#log_pos:U32.t{U32.v log_pos <= Seq.length log_bytes})
                      (#out_bytes:bytes)
+                     (#out_offset:U32.t)
                      (#out:A.array U8.t) //out array, to write outputs
                      (#aeh:AEH.aggregate_epoch_hashes) //lock & handle to the aggregate state
                      (res:U32.t)
    : STGhostT unit o
-     (verify_step_post tsm t log_bytes log_pos out_bytes out aeh (App_failure res))
+     (verify_step_post tsm t log_bytes log_pos out_bytes out_offset out aeh (App_failure res))
      (fun _ -> some_failure t out aeh)
    = rewrite
-        (verify_step_post tsm t log_bytes log_pos out_bytes out aeh (App_failure res))
+        (verify_step_post tsm t log_bytes log_pos out_bytes out_offset out aeh (App_failure res))
         (thread_state_inv t tsm `star`
          TLM.tid_pts_to aeh.mlogs tsm.thread_id full tsm.processed_entries false `star`
          array_pts_to out out_bytes);
@@ -631,15 +599,20 @@ let elim_verify_step_post_log_entry_failure
                      (#log_bytes:bytes)
                      (#log_pos:U32.t{U32.v log_pos <= Seq.length log_bytes})
                      (#out_bytes:bytes)
+                     (#out_offset:U32.t)
                      (#out:A.array U8.t) //out array, to write outputs
                      (#aeh:AEH.aggregate_epoch_hashes) //lock & handle to the aggregate state
                      (res:U32.t)
    : STGhostT unit o
-     (verify_step_post tsm t log_bytes log_pos out_bytes out aeh (Verify_entry_failure res))
+     (verify_step_post tsm t log_bytes log_pos out_bytes out_offset out aeh (Verify_entry_failure res))
      (fun _ -> some_failure t out aeh)
    = admit_()
 
-#push-options "--ifuel 0"
+#push-options "--ifuel 2"
+let rewrite_with #o (p q:vprop) (_ : squash (p == q))
+  : STGhostT unit o p (fun _ -> q)
+  = rewrite p q
+
 let stitch_verify_post_step
                    (#o:_)
                    (#tsm:M.thread_state_model)
@@ -658,30 +631,89 @@ let stitch_verify_post_step
                      (U32.v out_pos + U32.v out_pos') <= Seq.length out_bytes /\
                      UInt.fits (Seq.length log_bytes) 32 /\
                      UInt.fits (Seq.length out_bytes) 32)) o
-    (verify_step_post (M.verify_model tsm les) t log_bytes log_pos out_bytes_1 out aeh (Verify_success log_pos' out_pos'))
+    (verify_step_post (M.verify_model tsm les) t
+                      log_bytes log_pos
+                      out_bytes_1 out_pos out
+                      aeh (Verify_success log_pos' out_pos'))
     (fun _ ->
       verify_post tsm t log_bytes out_bytes out aeh
         (Verify_success U32.(log_pos +^ log_pos') U32.(out_pos +^ out_pos')))
     (requires
       parse_log_up_to log_bytes (U32.v log_pos) == Some les /\
-      Application.n_out_bytes tsm (M.verify_model tsm les) out_pos out_bytes out_bytes_1)
+      Application.n_out_bytes tsm (M.verify_model tsm les) 0ul out_pos out_bytes out_bytes_1)
     (ensures fun _ ->
       True)
-  = let le = elim_exists () in
+  = assume (UInt.fits (Seq.length log_bytes) 32 /\
+            UInt.fits (Seq.length out_bytes) 32);
+    let le = elim_exists () in
     elim_pure _;
     let out_bytes_2 = elim_exists () in
     elim_pure _;
+    assert_ (array_pts_to out out_bytes_2);
     let tsm1 = M.verify_model tsm les in
     let tsm2 = M.verify_step_model tsm1 le in
+    let les' = Seq.snoc les le in
+    assume (tsm2 == M.verify_model tsm les');
     rewrite (thread_state_inv t _)
-            (thread_state_inv t tsm2);
+            (thread_state_inv t (M.verify_model tsm les'));
     assume (tsm1.thread_id == tsm2.thread_id);
     rewrite (TLM.tid_pts_to _ _ _ _ _)
-            (TLM.tid_pts_to aeh.mlogs tsm2.thread_id full tsm2.processed_entries false);
-    assert_ (array_pts_to out out_bytes_2);
+            (TLM.tid_pts_to aeh.mlogs
+                            (M.verify_model tsm les').thread_id
+                            full
+                            (M.verify_model tsm les').processed_entries
+                            false);
+    assert (Application.n_out_bytes tsm1 tsm2 out_pos out_pos' out_bytes_1 out_bytes_2);
+    assume (Application.delta_out_bytes tsm tsm2 ==
+            Seq.append (Application.delta_out_bytes tsm tsm1)
+                       (Application.delta_out_bytes tsm1 tsm2));
+    intro_pure (Application.n_out_bytes
+                      tsm (M.verify_model tsm les')
+                      0ul U32.(out_pos +^ out_pos')
+                      out_bytes
+                      out_bytes_2);
+    intro_exists_erased out_bytes_2 (fun out_bytes_2 ->
+      array_pts_to out out_bytes_2 `star`
+      pure (Application.n_out_bytes
+                  tsm (M.verify_model tsm les')
+                  0ul U32.(out_pos +^ out_pos')
+                  out_bytes out_bytes_2));
+    rewrite_with
+      (exists_ (fun out_bytes_2 ->
+        array_pts_to out out_bytes_2 `star`
+        pure (Application.n_out_bytes
+                  tsm (M.verify_model tsm les')
+                  0ul U32.(out_pos +^ out_pos')
+                  out_bytes out_bytes_2)))
+      (verify_post_out_bytes tsm out_bytes U32.(out_pos +^ out_pos') out les')
+      (_ by FStar.Tactics.(
+        norm [delta_only [`%verify_post_out_bytes]];
+        trefl())
+      );
     assert (LogEntry.maybe_parse_log_entry log_bytes log_pos == Some (reveal le, U32.v log_pos'));
-    assert (Application.n_out_bytes tsm1 tsm2 out_pos' out_bytes_1 out_bytes_2);
-    admit_()
+    assume (parse_log_up_to log_bytes (U32.v log_pos) == Some les /\
+            LogEntry.maybe_parse_log_entry log_bytes log_pos == Some (reveal le, U32.v log_pos') ==>
+            parse_log_up_to log_bytes (U32.v log_pos + U32.v log_pos') == Some les');
+    intro_pure (parse_log_up_to log_bytes (U32.v (U32.(log_pos +^ log_pos'))) == Some les');
+    intro_exists les' (fun les' ->
+      pure (parse_log_up_to log_bytes (U32.v (U32.(log_pos +^ log_pos'))) == Some les') `star`
+      thread_state_inv t (M.verify_model tsm les') `star`
+      TLM.tid_pts_to aeh.mlogs
+                      (M.verify_model tsm les').thread_id
+                      full
+                      (M.verify_model tsm les').processed_entries
+                      false `star`
+      verify_post_out_bytes tsm out_bytes U32.(out_pos +^ out_pos') out les');
+     rewrite_with
+       (exists_ _)
+       (verify_post tsm t log_bytes out_bytes out aeh
+         (Verify_success U32.(log_pos +^ log_pos') U32.(out_pos +^ out_pos')))
+       (_ by FStar.Tactics.(
+         norm [delta_only [`%verify_post]; iota];
+         trefl())
+       );
+     ()
+
 #pop-options
 
 
@@ -730,13 +762,13 @@ let rec verify_log_ind
      A.pts_to_length out _;
      assume (not (M.verify_model tsm _log).failed);
      let res = verify_step t log_pos log out_pos out aeh in
-     assert_ (verify_step_post (M.verify_model tsm _log) t log_bytes log_pos _out_bytes_1 out aeh res);
+     assert_ (verify_step_post (M.verify_model tsm _log) t log_bytes log_pos _out_bytes_1 out_pos out aeh res);
      match res
            returns
              ST verify_result
                  (//precondition
                    A.pts_to log log_perm log_bytes `star`
-                   verify_step_post (M.verify_model tsm _log) t log_bytes log_pos _out_bytes_1 out aeh res)
+                   verify_step_post (M.verify_model tsm _log) t log_bytes log_pos _out_bytes_1 out_pos out aeh res)
                  (fun res' -> //postcondition
                    A.pts_to log log_perm log_bytes `star`
                    verify_post tsm t log_bytes out_bytes out aeh res')
@@ -772,9 +804,6 @@ let rec verify_log_ind
    )
 
 #push-options "--fuel 1"
-let rewrite_with #o (p q:vprop) (_ : squash (p == q))
-  : STGhostT unit o p (fun _ -> q)
-  = rewrite p q
 
 let intro_verify_post_success
                #o (#tsm:M.thread_state_model)
@@ -793,10 +822,10 @@ let intro_verify_post_success
      assume (Seq.length log_bytes > 0);
      assume (Application.delta_out_bytes tsm tsm == Seq.empty);
      intro_pure (parse_log_up_to log_bytes (U32.v 0ul) == Some les);
-     intro_pure (Application.n_out_bytes tsm (M.verify_model tsm les) 0ul out_bytes out_bytes);
+     intro_pure (Application.n_out_bytes tsm (M.verify_model tsm les) 0ul 0ul out_bytes out_bytes);
      intro_exists out_bytes (fun out_bytes1 ->
         array_pts_to out out_bytes1 `star`
-        pure (Application.n_out_bytes tsm (M.verify_model tsm les) 0ul out_bytes out_bytes1));
+        pure (Application.n_out_bytes tsm (M.verify_model tsm les) 0ul 0ul out_bytes out_bytes1));
      rewrite (thread_state_inv t tsm)
              (thread_state_inv t (M.verify_model tsm les));
      rewrite (TLM.tid_pts_to _ _ _ _ _)
@@ -809,7 +838,7 @@ let intro_verify_post_success
        TLM.tid_pts_to aeh.mlogs tsm'.thread_id full tsm'.processed_entries false `star`
        exists_ (fun out_bytes1 ->
          array_pts_to out out_bytes1 `star`
-         pure (Application.n_out_bytes tsm tsm' 0ul out_bytes out_bytes1)));
+         pure (Application.n_out_bytes tsm tsm' 0ul 0ul out_bytes out_bytes1)));
      rewrite_with (exists_ (fun log ->
        let tsm' = M.verify_model tsm log in
        pure (parse_log_up_to log_bytes (U32.v 0ul) == Some log) `star`
@@ -817,7 +846,7 @@ let intro_verify_post_success
        TLM.tid_pts_to aeh.mlogs tsm'.thread_id full tsm'.processed_entries false `star`
        exists_ (fun out_bytes1 ->
          array_pts_to out out_bytes1 `star`
-         pure (Application.n_out_bytes tsm tsm' 0ul out_bytes out_bytes1))))
+         pure (Application.n_out_bytes tsm tsm' 0ul 0ul out_bytes out_bytes1))))
        (verify_post tsm t log_bytes out_bytes out aeh (Verify_success 0ul 0ul))
        (_ by (FStar.Tactics.trefl()))
 
